cfg-list/reachGenGrammarScript.sml
@@ -7,24 +7,26 @@ generatingGrammarTheory;
 val _ = new_theory "reachGenGrammar";
 
 
-val rugr = Define `rugr g = G { rule l r | rule l r IN (rules (usefulnts g)) /\ ?a b.RTC (derives g) [NTS (startSym g)] (a++[NTS l]++b)} (startSym g)`;
+val rugr = Define `rugr g g' = 
+    ∃g0.usefulnts g g0 ∧
+    (∀e.MEM e (rules g') ⇔ 
+     e ∈ { rule l r | MEM (rule l r)  (rules g0) ∧ 
+	  ∃a b. RTC (derives g0) [NTS (startSym g0)] (a++[NTS l]++b) }) ∧
+    (startSym g = startSym g')`;
 
-val eq_srugr = prove (
-``startSym (rugr g) = startSym g``,
-Cases_on `g` THEN METIS_TAC [startSym_def,rugr]
-);
+
+val thm4_2 = store_thm
+("thm4_2",
+ ``~(language g = {}) ∧ (rugr g g') ⇒ (language g = language g')``,
+
+SRW_TAC [] [EQ_IMP_THM] THEN
+FULL_SIMP_TAC (srw_ss()) [rugr] THEN
+`language g = language g0`by METIS_TAC [lemma4_1a] THEN
+`rgr g0 g'` by 
+ (Cases_on `g` THEN
+  FULL_SIMP_TAC (srw_ss()) [rgr_def, usefulnts_def, startSym_def]) THEN
+METIS_TAC [thm4_2]);
 
 
-val thm4_2 = prove(
-``~(language g = {}) ==> (language g = language (rgr (usefulnts g)))``,
-SRW_TAC [] [language_def,EXTENSION,EQ_IMP_THM] 
-THENL[
-Cases_on `g` THEN
-FULL_SIMP_TAC (srw_ss()) [startSym_def,eq_startsym,eq_srgr] THEN
-`RTC (derives (usefulnts (G f s))) [NTS s] x'` by METIS_TAC [subr4] THEN
-METIS_TAC [rgr_r7,startSym_def,eq_srgr,eq_startsym],
-`RTC (derives (usefulnts g)) [NTS (startSym g)] x'` by METIS_TAC [rgr_subr3_rtc,startSym_def,eq_srgr,eq_startsym] THEN
-METIS_TAC [subr4_rev]
-]);
 
 val _ = export_theory ();
