cfg-list/unitProdsScript.sml
@@ -22,13 +22,13 @@ val nonUnitProds = Define
 `nonUnitProds g = (LIST_TO_SET (rules g)) DIFF (unitProds g)`;
 
 val newProds = Define 
-`newProds g p' = 
+`newProds (g:(α,β) grammar) (p':(α,β) rule -> bool) = 
 {rule a r | ∃b ru.(rule b r ∈ p' ∧ 
 		(NTS a,NTS b) IN allDeps (G ru (startSym g)) ∧
 		(∀e.MEM e ru = e ∈ (unitProds g)))}`;
 
 val upgr_rules = Define 
-`(upgr_rules g =  (nonUnitProds g) UNION (newProds g (nonUnitProds g)))`;
+`(upgr_rules g =  (nonUnitProds g) ∪ (newProds g (nonUnitProds g)))`;
 
 val upgr = Define 
 `upgr g g' = (∀e.MEM e (rules g') = e ∈ (upgr_rules g)) ∧
@@ -64,57 +64,56 @@ SRW_TAC [][nonUnitProds]);
 
 
 
-val g'ImpgRules = store_thm
-("g'ImpgRules",
-``e ∈ upgr_rules g ⇒ MEM e (rules g)``,
 
-SRW_TAC [][upgr_rules,nonUnitProds] THEN
- FULL_SIMP_TAC (srw_ss()) [newProds, unitProds, EXTENSION, allDeps] THEN
-SRW_TAC [][] THEN
-METIS_TAC [rule_11, rules_def]
+val gsubDeriv = store_thm
+("gsubDeriv",
+``(∀e.MEM e (rules g) ⇒ MEM e (rules g')) ⇒
+derives g v v' ⇒ derives g' v v'``,
 
+SRW_TAC [][derives_def] THEN
+METIS_TAC []);
 
-val upgr_r1 = prove 
-(``negr g0 g ⇒ upgr g g' ⇒
- derives g' v v' ⇒ 
- derives g v v'``,
- SRW_TAC [][] THEN
-FULL_SIMP_TAC (srw_ss()) [upgr,derives_def] THEN
-SRW_TAC [][] THEN
+val gsubRtcDeriv = store_thm
+("gsubRtcDeriv",
+``∀v v'.RTC (derives g) v v' ⇒ (∀e.MEM e (rules g) ⇒ MEM e (rules g')) ⇒
+ RTC (derives g') v v'``,
 
-
- );
-
-
-val upgr_r2 = prove(
-``∀u v.negr g0 g ⇒ upgr g g' ⇒
-RTC (derives g') u v ⇒ RTC (derives g) u v``,
-HO_MATCH_MP_TAC RTC_INDUCT_RIGHT1 THEN
-METIS_TAC [RTC_RULES,upgr_r1, RTC_SUBSET,RTC_RULES_RIGHT1]
-);
+HO_MATCH_MP_TAC RTC_STRONG_INDUCT THEN SRW_TAC [][] THEN
+METIS_TAC [RTC_RULES, gsubDeriv]);
 
 
 val upgr_r3 = prove
 (``∀v v'.negr g0 g ⇒ upgr g g' ⇒
 derives g' v v' ⇒ RTC (derives g) v v'``,
-MAGIC);
-
-(*
 
 SRW_TAC [] [derives_def, upgr, rules_def, nonUnitProds,newProds,allDeps,
 	    upgr_rules] 
 THENL[
  METIS_TAC [res1,derives_same_append_left,derives_same_append_right,RTC_SUBSET],
+
 Cases_on `g` THEN
-`RTC (derives g) [NTS lhs] [NTS b]` by MAGIC THEN
-`derives (negr (G f s)) [NTS b] rhs` by METIS_TAC [res1] THEN
+FULL_SIMP_TAC (srw_ss()) [startSym_def] THEN
+`∀e.e ∈ unitProds (G l n) ⇒ MEM e (rules (G l n))`
+      by  (FULL_SIMP_TAC (srw_ss()) [rules_def, unitProds, EXTENSION] THEN
+	   METIS_TAC []) THEN
+`RTC (derives (G l n)) [NTS lhs] [NTS b]` by METIS_TAC [gsubRtcDeriv, rules_def] THEN
+`derives (G l n) [NTS b] rhs` by METIS_TAC [res1] THEN
 FULL_SIMP_TAC (srw_ss()) [eq_sneup,startSym_def,rules_def] THEN
-`RTC (derives (negr (G f s))) [NTS lhs] rhs` 
+`RTC (derives (G l n)) [NTS lhs] rhs` 
       by METIS_TAC [RTC_RULES_RIGHT1,eq_sneup,eq_snegr,negr_def,
 		    rules_def] THEN
 METIS_TAC [rtc_derives_same_append_right,rtc_derives_same_append_left]
 ]);
-*)
+
+
+val upgr_r2 = prove(
+``∀u v.RTC (derives g') u v ⇒ negr g0 g ⇒ upgr g g' ⇒ RTC (derives g) u v``,
+HO_MATCH_MP_TAC RTC_INDUCT_RIGHT1 THEN
+SRW_TAC [][] THEN
+METIS_TAC [RTC_RULES,upgr_r3, RTC_RTC]
+);
+
+
 
 val upgr_r4 = store_thm("upgr_r4",
 ``∀u v.RTC (derives g') u v ⇒ 
@@ -146,28 +145,26 @@ val upgr_r6 = prove(
 (NTS x,NTS y) IN (allDeps g)``,
 SRW_TAC [] [allDeps] THEN SRW_TAC [] []);
 
+
 val negr_r16 = prove(
 ``∀v v'.negr g0 g ⇒ derives g v v' ⇒ ~(v'=[])``,
 SRW_TAC [] [] THEN
 FULL_SIMP_TAC (srw_ss()) [derives_def,negr_def,munge_def] THEN
-SRW_TAC [] []
-
-);
+SRW_TAC [][] THEN
+RES_TAC THEN
+FULL_SIMP_TAC (srw_ss()) []);
 
 
 val negr_r17 = prove(
-``rule l r IN rules (negr g) ⇒ ~(r=[])``,
-SRW_TAC [] [negr_runs,munge_def]);
+``negr g0 g ⇒ MEM (rule l r) (rules g) ⇒ ~(r=[])``,
+SRW_TAC [] [negr_def,munge_def]);
+
 
 val eqSymsToStr = Define 
 `(eqSyms (NTS nt1) (NTS nt2) = (nt1=nt2)) ∧
  (eqSyms (TS ts1) (TS ts2) = (ts1=ts2))`;
 
 
-(*
-val eqNTs = Define 
-`(eqNTs (nt1) (nt2) = (NTS nt1 = NTS nt2))`
-*)
 
 val rel_r1 = prove(
 ``∀x y.RTC R x y ∧ ~(x=y) ⇒ TC R x y``,
@@ -179,141 +176,170 @@ METIS_TAC [RTC_TRANSITIVE,TC_DEF]);
 
 
 val upgr_r8 = prove(
-``derives (negr g) [NTS lhs] [NTS nt] ⇒ derives (negr g) [NTS nt] r ⇒ ~(∃n.r=[NTS n]) ⇒ derives (upgr (negr g)) [NTS lhs] r``,
+``negr g0 g ⇒ upgr g g' ⇒
+derives g [NTS lhs] [NTS nt] ⇒ derives g [NTS nt] r ⇒ 
+		    ~(∃n.r=[NTS n]) ⇒ derives g' [NTS lhs] r``,
 SRW_TAC [] [] THEN
 FULL_SIMP_TAC (srw_ss()) [derives_def] THEN
 MAP_EVERY Q.EXISTS_TAC [`[]`,`[]`] THEN
 SRW_TAC [] [] THEN
-FULL_SIMP_TAC (srw_ss()) [upgr_runs] THEN
+FULL_SIMP_TAC (srw_ss()) [] THEN
 `(s1=[]) ∧ (s2=[]) ∧ (s1'=[]) ∧ (s2'=[])` by METIS_TAC [lres] THEN
 FULL_SIMP_TAC (srw_ss()) [] THEN
 SRW_TAC [] [] THEN
-SRW_TAC [] [upgr_runs] THEN
+FULL_SIMP_TAC (srw_ss()) [nonUnitProds,allDeps,newProds, upgr_rules,upgr] THEN
 DISJ2_TAC THEN
-SRW_TAC [] [nonUnitProds,allDeps,newProds ] THEN
 Q.EXISTS_TAC `lhs''` THEN
-SRW_TAC [] [] THENL[
- SRW_TAC [] [unitProds],
- MATCH_MP_TAC RTC_SUBSET THEN
-`derives (negr g) [NTS lhs] [NTS lhs'']` by METIS_TAC [res1] THEN
- SRW_TAC [] [unitProds,derives_def,rules_def] THEN
- METIS_TAC [APPEND]]);
+SRW_TAC [][] THEN
+MAGIC);
  
 
-val upgr_r9 = prove(
-``derives g' [NTS n] v 
-          ⇒ 
-    ∃nt. RTC (derives (G (unitProds g) (startSym g))) 
-               [NTS n] [NTS nt] ∧ derives g [NTS nt] v``,
+
+val upgr_r9 = prove
+(``upgr g0 g ⇒ derives g [NTS n] v ∧ (∀e.MEM e ru ⇔ e ∈ unitProds g0) ⇒
+∃nt. RTC (derives (G ru (startSym g0))) [NTS n] [NTS nt] ∧ 
+ derives g0 [NTS nt] v``,
+
 SRW_TAC [] [derives_def] THEN
 FULL_SIMP_TAC (srw_ss()) [lreseq] THEN
-SRW_TAC [][] THEN
-FULL_SIMP_TAC (srw_ss()) [upgr_runs] THENL[
-Q.EXISTS_TAC `lhs` THEN
-SRW_TAC [] [RTC_RULES] THEN
-FULL_SIMP_TAC (srw_ss()) [nonUnitProds] THEN
-MAP_EVERY Q.EXISTS_TAC [`[]`,`[]`,`rhs`,`lhs`] THEN
-SRW_TAC [] [],
-
-FULL_SIMP_TAC (srw_ss()) [newProds,allDeps] THEN
-Q.EXISTS_TAC `b` THEN
 SRW_TAC [] [] THEN
-FULL_SIMP_TAC (srw_ss()) [nonUnitProds]]);
+FULL_SIMP_TAC (srw_ss()) [upgr, upgr_rules] THEN 
+`rule lhs rhs ∈ nonUnitProds g0 ∨
+ rule lhs rhs ∈ newProds g0 (nonUnitProds g0)` by METIS_TAC [] 
+ THENL[
+       Q.EXISTS_TAC `lhs` THEN
+       SRW_TAC [] [RTC_RULES] THEN
+       FULL_SIMP_TAC (srw_ss()) [nonUnitProds] THEN
+       MAP_EVERY Q.EXISTS_TAC [`[]`,`[]`,`rhs`,`lhs`] THEN
+       SRW_TAC [] [],
+
+       FULL_SIMP_TAC (srw_ss()) [newProds,allDeps] THEN
+       Q.EXISTS_TAC `b` THEN
+       SRW_TAC [] [] THEN
+       `set ru = set ru'` by FULL_SIMP_TAC (srw_ss()) [EXTENSION] THEN
+       FULL_SIMP_TAC (srw_ss()) [nonUnitProds] THEN
+       METIS_TAC [rulesets_the_same_RTC_derives, IN_LIST_TO_SET, rules_def]
+       ]);
 
 
-val upgr_r10 = prove(
-``derives (negr g) [NTS nt1] [NTS nt2] ⇒ derives (G (unitProds (negr g)) (startSym (negr g))) [NTS nt1] [NTS nt2]``,
+val upgr_r10 = prove
+(``negr g0 g ⇒ derives g [NTS nt1] [NTS nt2] ∧
+(∀e.MEM e ru ⇔ e ∈ unitProds g) ⇒ 
+derives (G ru (startSym g)) [NTS nt1] [NTS nt2]``,
+
 SRW_TAC [] [] THEN
 FULL_SIMP_TAC (srw_ss()) [derives_def] THEN
 FULL_SIMP_TAC (srw_ss()) [lreseq] THEN
 SRW_TAC [] [rules_def,unitProds] THEN
 FULL_SIMP_TAC (srw_ss()) [] THEN
-SRW_TAC [] []);
+SRW_TAC [] []
+);
 
 
 val upgr_r12 = prove(
-``rule l r IN rules g' ⇒ ~(rule l r IN unitProds g)``,
-SRW_TAC [] [unitProds,upgr_runs] THENL[
+``upgr g0 g ⇒ MEM (rule l r) (rules g) ⇒ rule l r ∉ unitProds g0``,
+SRW_TAC [] [unitProds,upgr_rules, upgr] THENL[
 FULL_SIMP_TAC (srw_ss()) [nonUnitProds,unitProds] THEN METIS_TAC [],
-FULL_SIMP_TAC (srw_ss()) [newProds,nonUnitProds,allDeps,unitProds] THEN METIS_TAC []]);
+FULL_SIMP_TAC (srw_ss()) [newProds,nonUnitProds,allDeps,unitProds] THEN 
+METIS_TAC []]);
 
 
 
 val upgr_r13 = prove(
-``rule l r IN rules g' ⇒ ~(∃n.r=[NTS n])``,
+``upgr g0 g ⇒ MEM (rule l r) (rules g) ⇒ ∃n.r≠[NTS n]``,
 SRW_TAC [] [] THEN
-`~(rule l r IN unitProds g)` by METIS_TAC [upgr_r12]THEN
-FULL_SIMP_TAC (srw_ss()) [unitProds,upgr_runs] THENL[
-FULL_SIMP_TAC (srw_ss()) [nonUnitProds,unitProds] THEN METIS_TAC [],
-FULL_SIMP_TAC (srw_ss()) [nonUnitProds,newProds,allDeps,unitProds] THEN METIS_TAC []]);
+`rule l r ∉ unitProds g0` by METIS_TAC [upgr_r12] THEN
+FULL_SIMP_TAC (srw_ss()) [unitProds,upgr, upgr_rules] THEN
+RES_TAC
+THENL[
+      FULL_SIMP_TAC (srw_ss()) [nonUnitProds,unitProds] THEN
+      METIS_TAC [],
+      FULL_SIMP_TAC (srw_ss()) [nonUnitProds,newProds,allDeps,unitProds] THEN 
+      METIS_TAC []
+      ]);
 
 
 val upgr_r14 = prove(
-``derives (negr g) [NTS nt1] [NTS nt2] ⇒ derives (upgr (negr g)) [NTS nt2] v ⇒ derives (upgr (negr g)) [NTS nt1] v``,
-SRW_TAC [] [] THEN 
-`∃nt. RTC (derives (G (unitProds (negr g)) (startSym (negr g)))) [NTS nt2] [NTS nt] ∧ derives (negr g) [NTS nt] v` by METIS_TAC [upgr_r9] THEN
+``negr g0 g ⇒ derives g [NTS nt1] [NTS nt2] ⇒ upgr g g' ⇒
+derives g' [NTS nt2] v ⇒ derives g' [NTS nt1] v``,
 
-`derives (G (unitProds (negr g)) (startSym (negr g))) [NTS nt1] [NTS nt2]` by METIS_TAC [upgr_r10] THEN
-`RTC (derives (G (unitProds (negr g)) (startSym (negr g)))) [NTS nt1] [NTS nt]` by METIS_TAC [RTC_RULES] THEN
-SRW_TAC [] [derives_def,upgr_runs] THEN
-MAP_EVERY Q.EXISTS_TAC [`[]`,`[]`,`v`,`nt1`] THEN
-SRW_TAC [] [] THEN
-DISJ2_TAC THEN
-SRW_TAC [] [nonUnitProds,newProds,allDeps] THEN
-Q.EXISTS_TAC `nt` THEN
-SRW_TAC [] [] THENL[
-      FULL_SIMP_TAC (srw_ss()) [derives_def] THEN FULL_SIMP_TAC (srw_ss()) [lreseq] THEN SRW_TAC [] [],
-      FULL_SIMP_TAC (srw_ss()) [derives_def,lreseq] THEN
-`~ ∃n. v = [NTS n]` by METIS_TAC [upgr_r13] THEN SRW_TAC [] [unitProds]]);
+SRW_TAC [] [] THEN 
+`∃ru.∀e. e ∈ ru ⇔ e ∈ unitProds g` by MAGIC THEN
+IMP_RES_TAC upgr_r10 THEN
+IMP_RES_TAC upgr_r9 THEN
+`RTC (derives (G ru (startSym g))) [NTS nt1] [NTS nt]` 
+		     by METIS_TAC [RTC_RULES] THEN
+SRW_TAC [] [derives_def] THEN
+MAGIC);
 
 
 val up_r1 = prove (
-``rule lhs (s1++[NTS nt]++s2) IN unitProds g = (s1=[]) ∧ (s2=[]) ∧ rule lhs [NTS nt] IN unitProds g``,
+``rule lhs (s1++[NTS nt]++s2) ∈ unitProds g = 
+		   (s1=[]) ∧ (s2=[]) ∧ rule lhs [NTS nt] ∈ unitProds g``,
 SRW_TAC [][EQ_IMP_THM] THENL[
 
 FULL_SIMP_TAC (srw_ss()) [unitProds] THEN METIS_TAC [lres],
 
 FULL_SIMP_TAC (srw_ss()) [unitProds] THEN METIS_TAC [lres],
 
-FULL_SIMP_TAC (srw_ss()) [unitProds] THEN METIS_TAC [lres]]);
+FULL_SIMP_TAC (srw_ss()) [unitProds] THEN METIS_TAC [lres]
+]);
 
 
 val up_r2 = prove(
-``rule lhs rhs IN unitProds (negr g) ⇒ rule lhs rhs IN rules (negr g)``,
-SRW_TAC [] [unitProds]);
+``negr g0 g ⇒ rule lhs rhs ∈ unitProds g ⇒ MEM (rule lhs rhs) (rules g)``,
+SRW_TAC [] [unitProds]
+);
 
 val upgr_r20 = store_thm("upgr_r20",
-``∀u v.RTC (derives (negr g)) u v ⇒ EVERY isTmnlSym v ⇒ RTC (derives (upgr (negr g))) u v``,
+``∀u v.RTC (derives g) u v ⇒ negr g0 g ∧ upgr g g' ⇒ 
+		     EVERY isTmnlSym v ⇒ RTC (derives g') u v``,
+
 HO_MATCH_MP_TAC RTC_STRONG_INDUCT THEN
 SRW_TAC [] [RTC_RULES] THEN
 RES_TAC THEN
 FULL_SIMP_TAC (srw_ss()) [derives_def] THEN
-`∃s1' rhs' s2'. (v = s1' ++  rhs' ++ s2') ∧ RTC (derives (upgr(negr g))) s1 s1' ∧ RTC (derives (upgr (negr g))) rhs rhs' ∧ RTC (derives (upgr (negr g))) s2 s2'` by SRW_TAC [] [upgr_r19] THEN
+`∃s1' rhs' s2'. (v = s1' ++  rhs' ++ s2') ∧ RTC (derives g') s1 s1' ∧ 
+RTC (derives g') rhs rhs' ∧ RTC (derives g') s2 s2'` by SRW_TAC [] [upgr_r19] THEN
 FULL_SIMP_TAC (srw_ss()) [EVERY_APPEND] THEN
-`derives (negr g) [NTS lhs] rhs` by METIS_TAC [res1] THEN
-Cases_on `rhs=rhs'` THENL[
-  SRW_TAC [] [] THEN METIS_TAC [derives_append,upgr_r5,RTC_SUBSET,RTC_RULES,RTC_REFLEXIVE],
-  `∃sf.derives (upgr(negr g)) rhs sf ∧ RTC (derives (upgr (negr g))) sf rhs'` by METIS_TAC [rtc_r1] THEN
-  Cases_on `~(rule lhs rhs IN unitProds (negr g))` THENL[
-    SRW_TAC [] [] THEN   `rule lhs rhs IN rules (upgr(negr g))` by FULL_SIMP_TAC (srw_ss()) [unitProds,upgr_runs] THENL[
-      DISJ1_TAC THEN FULL_SIMP_TAC (srw_ss()) [nonUnitProds,unitProds] THEN METIS_TAC [RTC_SUBSET, res1, derives_append,RTC_RULES],
-      SRW_TAC [] [] THEN FULL_SIMP_TAC (srw_ss()) [derives_def] THEN SRW_TAC [] [] THEN 
-      METIS_TAC [res1,derives_same_append_right,derives_same_append_left,RTC_RULES]],
-   SRW_TAC [] [] THEN FULL_SIMP_TAC (srw_ss()) [derives_def] THEN SRW_TAC [] [] 
-   THEN  `(s1'''=[]) ∧ (s2'''=[]) ∧ rule lhs [NTS lhs''] IN unitProds (negr g)` by METIS_TAC [up_r1] THEN
-`rule lhs [NTS lhs''] IN rules (negr g)` by METIS_TAC [up_r2] THEN
-`derives (upgr (negr g)) [NTS lhs] rhs'''`by METIS_TAC [res1,upgr_r14] THEN FULL_SIMP_TAC (srw_ss()) [] THEN
-SRW_TAC [] [] THEN
-METIS_TAC [RTC_RULES,derives_append]]]);
+`derives g [NTS lhs] rhs` by METIS_TAC [res1] THEN
+Cases_on `rhs=rhs'` 
+THENL[
+      SRW_TAC [] [] THEN 
+      METIS_TAC [derives_append,upgr_r5,RTC_SUBSET,RTC_RULES,RTC_REFLEXIVE],
+
+      `∃sf.derives g' rhs sf ∧ RTC (derives g') sf rhs'` by METIS_TAC [rtc_r1] THEN
+      Cases_on `rule lhs rhs ∉ unitProds g` 
+      THENL[
+	    SRW_TAC [] [] THEN   
+	    `MEM (rule lhs rhs) (rules g')` 
+	    by (FULL_SIMP_TAC (srw_ss()) [unitProds, upgr, upgr_rules,
+					  nonUnitProds]  THEN
+		METIS_TAC []) THEN
+	    FULL_SIMP_TAC (srw_ss()) [nonUnitProds,unitProds] THEN 
+	    METIS_TAC [RTC_SUBSET, res1, derives_append,RTC_RULES],
+		  
+
+	    SRW_TAC [] [] THEN FULL_SIMP_TAC (srw_ss()) [derives_def] THEN 
+	    SRW_TAC [] [] THEN  
+	    `(s1'''=[]) /\ (s2'''=[]) /\ rule lhs [NTS lhs''] ∈ unitProds g` 
+	    by METIS_TAC [up_r1] THEN
+	    `MEM (rule lhs [NTS lhs'']) (rules g)` by METIS_TAC [up_r2] THEN
+	    `derives g' [NTS lhs] rhs'''` by METIS_TAC [res1,upgr_r14] THEN 
+	    FULL_SIMP_TAC (srw_ss()) [] THEN
+	    SRW_TAC [] [] THEN
+	    METIS_TAC [RTC_RULES,derives_append]]]);
 
 
 
 val thm4_4 = store_thm("thm4_4",
-``~([] IN language g) ⇒ (language (negr g) = language (upgr (negr g)))``,
+``[] ∉ language g ∧ negr g0 g ∧ upgr g g' ⇒ 
+		   (language g = language g')``,
 SRW_TAC [] [language_def,EXTENSION,EQ_IMP_THM]
 THENL[
 METIS_TAC [upgr_r20,eq_supgr],
-METIS_TAC [upgr_r4,eq_supgr]])
+METIS_TAC [upgr_r4,eq_supgr]
+]);
 
 
 val _ = export_theory ();
